git-svn-id: orca@161

WP1-Programming-Languages-Semantics/WP11-C-semantics/src/IMP-Lenses/Commands.thy
@@ -65,7 +65,7 @@ by (metis det single_valued_def some_equality)
 definition W :: "('\<sigma> \<Rightarrow> bool) \<Rightarrow>('\<sigma> \<times> '\<sigma>) set \<Rightarrow> (('\<sigma> \<times> '\<sigma>) set \<Rightarrow> ('\<sigma> \<times> '\<sigma>) set)" 
 where     "W b cd = (\<lambda>cw. {(s,t). if b s then (s, t) \<in> cd O cw else s = t})"
 
-abbreviation While :: "('\<alpha> \<Rightarrow> bool) \<Rightarrow> '\<alpha> states \<Rightarrow> '\<alpha> states"  ("WHILE (_) DO /(_) OD"  70) where
+definition While :: "('\<alpha> \<Rightarrow> bool) \<Rightarrow> '\<alpha> states \<Rightarrow> '\<alpha> states"  ("WHILE (_) DO /(_) OD"  70) where
 "While Bexp Body \<equiv> (RelInv(lfp(W Bexp (Rel Body))))" (*emm...*)
 
 
