WP1-Programming-Languages-Semantics/WP11-C-semantics/src/SIMPL-Lenses/Substitution.thy
@@ -95,7 +95,7 @@ lemma usubst_upd_comm2:
 
 lemma usubst_upd_var_id [states]: 
   assumes "vwb_lens x"
-  shows "[x \<mapsto>\<^sub>s imp_var x] = id"
+  shows "[x \<mapsto>\<^sub>s VAR x] = id"
   using assms unfolding subst_upd_var_def
   by transfer (rule ext,auto)
 
